theories/Examples.v
@@ -1,0 +1,46 @@
+Require Import List.
+Require Import Autosubst.Autosubst.
+Require Import Coq.Relations.Relation_Definitions.
+
+Require Import LambdaM Canonical.
+
+
+Lemma mmap_append {A: Type} (f: A -> A) (l1 l2: list A) :
+  mmap f (l1 ++ l2) = (mmap f l1) ++ (mmap f l2).
+Proof.
+  induction l1 ; asimpl ; try rewrite IHl1 ; auto.
+Qed.
+
+Lemma step_subst :
+  (forall s t, LambdaM.step s t -> forall σ, LambdaM.step s.[σ] t.[σ])
+  /\
+  (forall l l', LambdaM.step' l l' -> forall σ, LambdaM.step' l..[σ] l'..[σ]) .
+Proof.
+  apply LambdaM.mut_comp_ind ; intros ; asimpl ;
+    try (constructor ; apply H). 
+  
+  - destruct b as [Beta | H].
+    + destruct Beta as [Beta1 | Beta2].
+      * induction Beta1. subst.
+        constructor. left. left. constructor. autosubst.
+      * induction Beta2. subst.
+        constructor. left. right. constructor. autosubst.
+    + induction H. subst.
+      constructor. right. constructor. auto.
+Qed.
+
+Lemma step_subst_can :
+  (forall s t, Canonical.step s t -> forall σ, Canonical.step s.[σ] t.[σ])
+  /\
+  (forall l l', Canonical.step' l l' -> forall σ, Canonical.step' l..[σ] l' ..[σ]).
+Proof.
+  apply Canonical.mut_comp_ind ; intros ; autounfold ; asimpl ;
+    try (now constructor ; apply H).
+
+  - apply step_comp_app2. apply H.
+  - apply step_comp_app3. apply H.
+  - destruct b as [Beta1 | Beta2] ; constructor.
+    + induction Beta1. subst. left. constructor. autosubst.
+    + induction Beta2. subst. right. asimpl. constructor.
+      rewrite app_subst_comm. f_equal. autosubst.
+Qed.
